f.v
@@ -43,17 +43,612 @@ Module exprop.
 End exprop.
 
 Module type.
-   Include abt.abt tyop.
-   Notation arrow ty1 ty2 := (op tyop.arrow [bind 0 ty1; bind 0 ty2]).
-   Notation all ty := (op tyop.all [bind 1 ty]).
+  Module A := abt.internal tyop.
+
+  Inductive t :=
+  | var (alpha : nat) : t
+  | arrow : t -> t -> t
+  | all : t -> t
+  .
+
+  Fixpoint to_abt (ty : t) : A.t :=
+    match ty with
+    | var n => A.var n
+    | arrow ty1 ty2 => A.op tyop.arrow [A.bind 0 (to_abt ty1); A.bind 0 (to_abt ty2)]
+    | all ty' => A.op tyop.all [A.bind 1 (to_abt ty')]
+    end.
+
+  Fixpoint of_abt (a : A.t) : t :=
+    match a with
+    | A.var n => var n
+    | A.op tyop.arrow [A.bind 0 a1; A.bind 0 a2] => arrow (of_abt a1) (of_abt a2)
+    | A.op tyop.all [A.bind 1 a'] => all (of_abt a')
+    | _ => var 0 (* bogus *)
+    end.
+
+  Lemma ws_to_abt : forall ty, A.ws (to_abt ty).
+  Proof. induction ty; simpl; intuition. Qed.
+
+  Lemma of_to_abt : forall ty, of_abt (to_abt ty) = ty.
+  Proof. induction ty; simpl; f_equal; auto. Qed.
+
+  Lemma to_of_abt : forall a, A.ws a -> to_abt (of_abt a) = a.
+  Proof.
+    induction a using A.rect'
+    with (Pb := fun b => forall v,
+                    A.ws_binder v b ->
+                    match b with
+                    | A.bind _ a => to_abt (of_abt a) = a
+                    end) ; simpl; intros; f_equal; intuition;
+      fold A.ws_binders in *.
+    - repeat break_match; subst; simpl in *; intuition;
+        repeat match goal with
+               | [ H : Forall _ (_ :: _) |- _ ] => inversion H; subst; clear H
+               end; simpl in *; try omega;
+      repeat f_equal; eauto.
+  Qed.
+
+  Fixpoint shift c d (ty : t) : t :=
+    match ty with
+    | var alpha => var (if alpha <? c then alpha else alpha + d)
+    | arrow ty1 ty2 => arrow (shift c d ty1) (shift c d ty2)
+    | all ty' => all (shift (S c) d ty')
+    end.
+
+  Lemma shift_to_of_abt : forall ty c d, shift c d ty = of_abt (A.shift c d (to_abt ty)).
+  Proof. induction ty; simpl; intros c d; f_equal; auto. Qed.
+    
+  Fixpoint subst rho ty :=
+    match ty with
+    | var alpha => match nth_error rho alpha with
+                  | Some ty' => ty'
+                  | None => ty
+                  end
+    | arrow ty1 ty2 => arrow (subst rho ty1) (subst rho ty2)
+    | all ty' => all (subst (var 0 :: map (shift 0 1) rho) ty')
+    end.
+
+  Hint Resolve A.ws_shift ws_to_abt.
+
+  Lemma shift_to_abt_comm : forall ty c d, to_abt (shift c d ty) = A.shift c d (to_abt ty).
+  Proof. intros. rewrite shift_to_of_abt, to_of_abt; auto. Qed.
+
+  Lemma map_shift_to_abt_comm :
+    forall c d rho, map to_abt (map (shift c d) rho) = map (A.shift c d) (map to_abt rho).
+  Proof.
+    intros.
+    rewrite !map_map.
+    now erewrite map_ext by (intros; apply shift_to_abt_comm).
+  Qed.
+  
+  Lemma subst_to_of_abt :
+    forall ty rho,
+      subst rho ty = of_abt (A.subst (map to_abt rho) (to_abt ty)).
+  Proof.
+    induction ty; simpl; intros rho; try rewrite ?A.descend_0, ?A.descend_1; f_equal; auto.
+    - rewrite nth_error_map.
+      break_match; auto.
+      now rewrite of_to_abt.
+    - rewrite IHty. simpl.
+      now rewrite map_shift_to_abt_comm.
+  Qed.
+
+  Fixpoint wf n ty :=
+    match ty with
+    | var alpha => alpha < n
+    | arrow ty1 ty2 => wf n ty1 /\ wf n ty2
+    | all ty' => wf (S n) ty'
+    end.
+
+  Lemma wf_to_abt : forall ty n, wf n ty <-> A.wf n (to_abt ty).
+  Proof. induction ty; simpl; firstorder. Qed.
+
+  Lemma wf_of_abt :
+    forall a n,
+      A.ws a -> 
+      wf n (of_abt a) <-> A.wf n a.
+  Proof.
+    intros.
+    pose proof wf_to_abt (of_abt a) n.
+    rewrite to_of_abt in *; auto.
+  Qed.
+
+  Fixpoint identity_subst (n : nat) : list t :=
+    match n with
+    | 0 => []
+    | S n => var 0 :: map (shift 0 1) (identity_subst n)
+    end.
+
+  Lemma shift_of_abt_comm :
+    forall a c d,
+      A.ws a -> 
+      shift c d (of_abt a) = of_abt (A.shift c d a).
+  Proof.
+    intros a c d WS.
+    rewrite shift_to_of_abt.
+    now rewrite to_of_abt by assumption.
+  Qed.
+
+  Lemma map_shift_of_abt_comm :
+    forall rho c d,
+      Forall A.ws rho -> 
+      map (shift c d) (map of_abt rho) = map of_abt (map (A.shift c d) rho).
+  Proof.
+    intros rho c d WS.
+    rewrite !map_map.
+    apply map_ext_in.
+    intros a I.
+    rewrite shift_of_abt_comm; auto.
+    eapply Forall_forall; eauto.
+  Qed.
+
+  Lemma identity_subst_of_abt :
+    forall n,
+      identity_subst n = List.map of_abt (A.identity_subst n).
+  Proof.
+    induction n; simpl; f_equal; auto.
+    rewrite IHn.
+    rewrite map_shift_of_abt_comm; auto.
+    apply A.ws_identity_subst.
+  Qed.
+
+  Lemma wf_shift : forall ty c d n, wf n ty -> wf (d + n) (shift c d ty).
+  Proof.
+    intros.
+    rewrite shift_to_of_abt.
+    rewrite wf_of_abt; auto.
+    apply A.wf_shift.
+    now rewrite <- wf_to_abt.
+  Qed.
+
+  Lemma wf_subst : forall ty n rho, wf (length rho) ty -> Forall (wf n) rho -> wf n (subst rho ty).
+  Proof.
+    intros ty n rho WF F.
+    rewrite subst_to_of_abt.
+    rewrite wf_of_abt.
+    - apply A.wf_subst.
+      + now rewrite map_length, <- wf_to_abt.
+      + rewrite Forall_map.
+        eapply Forall_impl; try eassumption.
+        intros ty' WF'.
+        now rewrite <- wf_to_abt.
+    - apply A.ws_subst; auto.
+      rewrite Forall_map.
+      apply Forall_forall; auto.
+  Qed.
+
+  Lemma identity_subst_length : forall n, length (identity_subst n) = n.
+  Proof.
+    intros.
+    rewrite identity_subst_of_abt.
+    rewrite map_length.
+    apply A.identity_subst_length.
+  Qed.
+
+  Lemma wf_identity_subst: forall n : nat, Forall (wf n) (identity_subst n).
+  Proof.
+    intros.
+    rewrite identity_subst_of_abt.
+    rewrite Forall_map.
+    rewrite Forall_forall.
+    intros ty I.
+    rewrite wf_of_abt.
+    - eapply Forall_forall; [apply A.wf_identity_subst|]; auto.
+    - eapply Forall_forall; [apply A.ws_identity_subst|]; eauto.
+  Qed.
+
+  Lemma wf_weaken : forall ty n d, n <= d -> wf n ty -> wf d ty.
+  Proof.
+    intros ty n d LE.
+    rewrite !wf_to_abt.
+    eauto using A.wf_weaken.
+  Qed.
+
+  Lemma shift_merge : forall ty c d1 d2 , shift c d2 (shift c d1 ty) = shift c (d2 + d1) ty.
+  Proof.
+    intros ty c d1 d2.
+    rewrite !shift_to_of_abt.
+    rewrite to_of_abt by auto.
+    now rewrite A.shift_merge.
+  Qed.
+
+  Lemma shift_nop_d :
+    forall ty c,
+      shift c 0 ty = ty.
+  Proof.
+    intros ty c.
+    rewrite shift_to_of_abt.
+    rewrite A.shift_nop_d.
+    now rewrite of_to_abt.
+  Qed.
+
+  Lemma subst_to_abt_comm : forall ty rho, to_abt (subst rho ty) = A.subst (map to_abt rho) (to_abt ty).
+  Proof.
+    intros. rewrite subst_to_of_abt, to_of_abt; auto.
+    apply A.ws_subst; auto.
+    rewrite Forall_map.
+    apply Forall_forall.
+    auto.
+  Qed.
+
+  Lemma map_subst_to_abt_comm :
+    forall rho1 rho2,
+      map to_abt (map (subst rho2) rho1) =
+      map (A.subst (map to_abt rho2)) (map to_abt rho1).
+  Proof.
+    intros rho1 rho2.
+    rewrite !map_map.
+    apply map_ext.
+    intros ty'.
+    auto using subst_to_abt_comm.
+  Qed.
+
+  Lemma subst_subst :
+    forall ty rho1 rho2,
+      wf (List.length rho1) ty ->
+      List.Forall (wf (List.length rho2)) rho1 ->
+      subst rho2 (subst rho1 ty) =
+      subst (List.map (subst rho2) rho1) ty.
+  Proof.
+    intros ty rho1 rho2 WF F.
+    rewrite !subst_to_of_abt.
+    rewrite !to_of_abt.
+    - rewrite A.subst_subst.
+      + now rewrite map_subst_to_abt_comm.
+      + now rewrite map_length, <- wf_to_abt.
+      + rewrite map_length, Forall_map.
+        eapply Forall_impl; try eassumption.
+        intros ty'.
+        now rewrite wf_to_abt.
+    - apply A.ws_subst; auto.
+      rewrite Forall_map.
+      apply Forall_forall; auto.
+  Qed.
+
+  Lemma subst_shift_singleton :
+    forall ty ty',
+      wf 0 ty ->
+      subst [ty'] (shift 0 1 ty) = ty.
+  Proof.
+    intros.
+    rewrite subst_to_of_abt, shift_to_of_abt.
+    simpl.
+    rewrite to_of_abt.
+    - rewrite A.subst_shift_singleton.
+      + now rewrite of_to_abt.
+      + now rewrite <- wf_to_abt.
+    - apply A.ws_shift; auto.
+  Qed.
+
+  Lemma subst_identity :
+    forall ty n,
+      subst (identity_subst n) ty = ty.
+  Proof.
+    intros ty n.
+    rewrite subst_to_of_abt, identity_subst_of_abt.
+    rewrite !map_map.
+    erewrite map_ext_in.
+    rewrite map_id.
+    rewrite A.subst_identity.
+    now rewrite of_to_abt.
+    intros ty' I.
+    simpl.
+    rewrite to_of_abt; auto.
+    eapply Forall_forall.
+    apply A.ws_identity_subst.
+    eauto.
+  Qed.
+
 End type.
 
 Module expr.
-   Include abt.abt exprop.
-   Notation abs e := (op exprop.abs [bind 1 e]).
-   Notation app e1 e2 := (op exprop.app [bind 0 e1; bind 0 e2]).
-   Notation tyabs e := (op exprop.tyabs [bind 0 e]).
-   Notation tyapp e := (op exprop.tyapp [bind 0 e]).
+  Module A := abt.internal exprop.
+
+  Inductive t :=
+  | var (x : nat) : t
+  | abs : t -> t
+  | app : t -> t -> t
+  | tyabs : t -> t
+  | tyapp : t -> t
+  .
+
+  Fixpoint to_abt (ty : t) : A.t :=
+    match ty with
+    | var n => A.var n
+    | abs e' => A.op exprop.abs [A.bind 1 (to_abt e')]
+    | app e1 e2 => A.op exprop.app [A.bind 0 (to_abt e1); A.bind 0 (to_abt e2)]
+    | tyabs e' => A.op exprop.tyabs [A.bind 0 (to_abt e')] 
+    | tyapp e' => A.op exprop.tyapp [A.bind 0 (to_abt e')]
+    end.
+
+  Fixpoint of_abt (a : A.t) : t :=
+    match a with
+    | A.var n => var n
+    | A.op exprop.abs [A.bind 1 a'] => abs (of_abt a')
+    | A.op exprop.app [A.bind 0 a1; A.bind 0 a2] => app (of_abt a1) (of_abt a2)
+    | A.op exprop.tyabs [A.bind 0 a'] => tyabs (of_abt a')
+    | A.op exprop.tyapp [A.bind 0 a'] => tyapp (of_abt a')
+    | _ => var 0 (* bogus *)
+    end.
+
+  Lemma ws_to_abt : forall e, A.ws (to_abt e).
+  Proof. induction e; simpl; intuition. Qed.
+
+  Lemma of_to_abt : forall e, of_abt (to_abt e) = e.
+  Proof. induction e; simpl; f_equal; auto. Qed.
+
+  Lemma to_of_abt : forall a, A.ws a -> to_abt (of_abt a) = a.
+  Proof.
+    induction a using A.rect'
+    with (Pb := fun b => forall v,
+                    A.ws_binder v b ->
+                    match b with
+                    | A.bind _ a => to_abt (of_abt a) = a
+                    end) ; simpl; intros; f_equal; intuition;
+      fold A.ws_binders in *.
+    - repeat break_match; subst; simpl in *; intuition;
+        repeat match goal with
+               | [ H : Forall _ (_ :: _) |- _ ] => inversion H; subst; clear H
+               end; simpl in *; try omega;
+      repeat f_equal; eauto.
+  Qed.
+
+  Fixpoint shift c d (e : t) : t :=
+    match e with
+    | var x => var (if x <? c then x else x + d)
+    | abs e' => abs (shift (S c) d e')
+    | app e1 e2 => app (shift c d e1) (shift c d e2)
+    | tyabs e' => tyabs (shift c d e')
+    | tyapp e' => tyapp (shift c d e')
+    end.
+
+  Lemma shift_to_of_abt : forall e c d, shift c d e = of_abt (A.shift c d (to_abt e)).
+  Proof. induction e; simpl; intros c d; f_equal; auto. Qed.
+    
+  Fixpoint subst rho e :=
+    match e with
+    | var x => match nth_error rho x with
+                  | Some e' => e'
+                  | None => e
+                  end
+    | abs e' => abs (subst (var 0 :: map (shift 0 1) rho) e')
+    | app e1 e2 => app (subst rho e1) (subst rho e2)
+    | tyabs e' => tyabs (subst rho e')
+    | tyapp e' => tyapp (subst rho e')
+    end.
+
+  Hint Resolve A.ws_shift ws_to_abt.
+
+  Lemma shift_to_abt_comm : forall e c d, to_abt (shift c d e) = A.shift c d (to_abt e).
+  Proof. intros. rewrite shift_to_of_abt, to_of_abt; auto. Qed.
+
+  Lemma map_shift_to_abt_comm :
+    forall c d rho, map to_abt (map (shift c d) rho) = map (A.shift c d) (map to_abt rho).
+  Proof.
+    intros.
+    rewrite !map_map.
+    now erewrite map_ext by (intros; apply shift_to_abt_comm).
+  Qed.
+  
+  Lemma subst_to_of_abt :
+    forall e rho,
+      subst rho e = of_abt (A.subst (map to_abt rho) (to_abt e)).
+  Proof.
+    induction e; simpl; intros rho; try rewrite ?A.descend_0, ?A.descend_1; f_equal; auto.
+    - rewrite nth_error_map.
+      break_match; auto.
+      now rewrite of_to_abt.
+    - rewrite IHe. simpl.
+      now rewrite map_shift_to_abt_comm.
+  Qed.
+
+  Fixpoint wf n e :=
+    match e with
+    | var x => x < n
+    | abs e' => wf (S n) e'
+    | app e1 e2 => wf n e1 /\ wf n e2
+    | tyabs e' => wf n e'
+    | tyapp e' => wf n e'
+    end.
+
+  Lemma wf_to_abt : forall e n, wf n e <-> A.wf n (to_abt e).
+  Proof. induction e; simpl; firstorder. Qed.
+
+  Lemma wf_of_abt :
+    forall a n,
+      A.ws a -> 
+      wf n (of_abt a) <-> A.wf n a.
+  Proof.
+    intros.
+    pose proof wf_to_abt (of_abt a) n.
+    rewrite to_of_abt in *; auto.
+  Qed.
+
+  Fixpoint identity_subst (n : nat) : list t :=
+    match n with
+    | 0 => []
+    | S n => var 0 :: map (shift 0 1) (identity_subst n)
+    end.
+
+  Lemma shift_of_abt_comm :
+    forall a c d,
+      A.ws a -> 
+      shift c d (of_abt a) = of_abt (A.shift c d a).
+  Proof.
+    intros a c d WS.
+    rewrite shift_to_of_abt.
+    now rewrite to_of_abt by assumption.
+  Qed.
+
+  Lemma map_shift_of_abt_comm :
+    forall rho c d,
+      Forall A.ws rho -> 
+      map (shift c d) (map of_abt rho) = map of_abt (map (A.shift c d) rho).
+  Proof.
+    intros rho c d WS.
+    rewrite !map_map.
+    apply map_ext_in.
+    intros a I.
+    rewrite shift_of_abt_comm; auto.
+    eapply Forall_forall; eauto.
+  Qed.
+
+  Lemma identity_subst_of_abt :
+    forall n,
+      identity_subst n = List.map of_abt (A.identity_subst n).
+  Proof.
+    induction n; simpl; f_equal; auto.
+    rewrite IHn.
+    rewrite map_shift_of_abt_comm; auto.
+    apply A.ws_identity_subst.
+  Qed.
+
+  Lemma wf_shift : forall e c d n, wf n e -> wf (d + n) (shift c d e).
+  Proof.
+    intros.
+    rewrite shift_to_of_abt.
+    rewrite wf_of_abt; auto.
+    apply A.wf_shift.
+    now rewrite <- wf_to_abt.
+  Qed.
+
+  Lemma wf_subst : forall e n rho, wf (length rho) e -> Forall (wf n) rho -> wf n (subst rho e).
+  Proof.
+    intros e n rho WF F.
+    rewrite subst_to_of_abt.
+    rewrite wf_of_abt.
+    - apply A.wf_subst.
+      + now rewrite map_length, <- wf_to_abt.
+      + rewrite Forall_map.
+        eapply Forall_impl; try eassumption.
+        intros e' WF'.
+        now rewrite <- wf_to_abt.
+    - apply A.ws_subst; auto.
+      rewrite Forall_map.
+      apply Forall_forall; auto.
+  Qed.
+
+  Lemma identity_subst_length : forall n, length (identity_subst n) = n.
+  Proof.
+    intros.
+    rewrite identity_subst_of_abt.
+    rewrite map_length.
+    apply A.identity_subst_length.
+  Qed.
+
+  Lemma wf_identity_subst: forall n : nat, Forall (wf n) (identity_subst n).
+  Proof.
+    intros.
+    rewrite identity_subst_of_abt.
+    rewrite Forall_map.
+    rewrite Forall_forall.
+    intros e I.
+    rewrite wf_of_abt.
+    - eapply Forall_forall; [apply A.wf_identity_subst|]; auto.
+    - eapply Forall_forall; [apply A.ws_identity_subst|]; eauto.
+  Qed.
+
+  Lemma wf_weaken : forall e n d, n <= d -> wf n e -> wf d e.
+  Proof.
+    intros e n d LE.
+    rewrite !wf_to_abt.
+    eauto using A.wf_weaken.
+  Qed.
+
+  Lemma shift_merge : forall e c d1 d2 , shift c d2 (shift c d1 e) = shift c (d2 + d1) e.
+  Proof.
+    intros e c d1 d2.
+    rewrite !shift_to_of_abt.
+    rewrite to_of_abt by auto.
+    now rewrite A.shift_merge.
+  Qed.
+
+  Lemma shift_nop_d :
+    forall e c,
+      shift c 0 e = e.
+  Proof.
+    intros e c.
+    rewrite shift_to_of_abt.
+    rewrite A.shift_nop_d.
+    now rewrite of_to_abt.
+  Qed.
+
+  Lemma subst_to_abt_comm : forall e rho, to_abt (subst rho e) = A.subst (map to_abt rho) (to_abt e).
+  Proof.
+    intros. rewrite subst_to_of_abt, to_of_abt; auto.
+    apply A.ws_subst; auto.
+    rewrite Forall_map.
+    apply Forall_forall.
+    auto.
+  Qed.
+
+  Lemma map_subst_to_abt_comm :
+    forall rho1 rho2,
+      map to_abt (map (subst rho2) rho1) =
+      map (A.subst (map to_abt rho2)) (map to_abt rho1).
+  Proof.
+    intros rho1 rho2.
+    rewrite !map_map.
+    apply map_ext.
+    intros e'.
+    auto using subst_to_abt_comm.
+  Qed.
+
+  Lemma subst_subst :
+    forall e rho1 rho2,
+      wf (List.length rho1) e ->
+      List.Forall (wf (List.length rho2)) rho1 ->
+      subst rho2 (subst rho1 e) =
+      subst (List.map (subst rho2) rho1) e.
+  Proof.
+    intros e rho1 rho2 WF F.
+    rewrite !subst_to_of_abt.
+    rewrite !to_of_abt.
+    - rewrite A.subst_subst.
+      + now rewrite map_subst_to_abt_comm.
+      + now rewrite map_length, <- wf_to_abt.
+      + rewrite map_length, Forall_map.
+        eapply Forall_impl; try eassumption.
+        intros e'.
+        now rewrite wf_to_abt.
+    - apply A.ws_subst; auto.
+      rewrite Forall_map.
+      apply Forall_forall; auto.
+  Qed.
+
+  Lemma subst_shift_singleton :
+    forall e e',
+      wf 0 e ->
+      subst [e'] (shift 0 1 e) = e.
+  Proof.
+    intros.
+    rewrite subst_to_of_abt, shift_to_of_abt.
+    simpl.
+    rewrite to_of_abt.
+    - rewrite A.subst_shift_singleton.
+      + now rewrite of_to_abt.
+      + now rewrite <- wf_to_abt.
+    - apply A.ws_shift; auto.
+  Qed.
+
+  Lemma subst_identity :
+    forall e n,
+      subst (identity_subst n) e = e.
+  Proof.
+    intros e n.
+    rewrite subst_to_of_abt, identity_subst_of_abt.
+    rewrite !map_map.
+    erewrite map_ext_in.
+    rewrite map_id.
+    rewrite A.subst_identity.
+    now rewrite of_to_abt.
+    intros e' I.
+    simpl.
+    rewrite to_of_abt; auto.
+    eapply Forall_forall.
+    apply A.ws_identity_subst.
+    eauto.
+  Qed.
 End expr.
 
 Module has_type.
@@ -86,23 +681,17 @@ Module has_type.
       Forall (type.wf n) G ->
       type.wf n ty.
   Proof.
-    induction 1; simpl in *; intuition.
+    induction 1; cbn in *; intuition.
     - now eapply Forall_nth; eauto.
     - apply IHt.
       rewrite Forall_map.
-      eapply Forall_impl; [|now eauto].
-      intros e' WF.
-      now apply type.wf_shift with (c := 0) (d := 1).
+      eapply Forall_impl; try eassumption.
+      intros ty' WF'.
+      now apply type.wf_shift with (d := 1).
     - apply type.wf_subst.
-      + simpl. now rewrite type.identity_subst_length.
+      + simpl. now rewrite type.identity_subst_length in *.
       + constructor; auto.
-        clear H H0 H1 H3 H4.
-        induction n; simpl; constructor.
-        * simpl. omega.
-        * rewrite Forall_map.
-          eapply Forall_impl; [|now eauto].
-          intros e' WF'.
-          now apply type.wf_shift with (c := 0) (d := 1).
+        apply type.wf_identity_subst.
   Qed.
 
   Lemma t_expr_wf :
